type_system/type_aux_lemmas.v
@@ -832,7 +832,7 @@ destruct orig. destruct H2.
   clear VL CL HL RL JL WFHL WFFL WFIL.
   simpl in *. eapply ExistsEl. eapply IH1. auto.
   rewrite hyp_shift_comm, form_shift_comm; aomega.
-+ specialize (JL _ _ _ H2 A_ins (S i)) as IH1.
++ specialize (JL _ _ _ H3 A_ins (S i)) as IH1.
   assert (
   forall op Aop Bop,
      get_op_type Σ op = Some (Aop, Bop) ->
@@ -846,13 +846,14 @@ destruct orig. destruct H2.
           (form_subs (form_shift φ 2 0) 2 
             (Fun TyUnit (Op op Aop Bop (Var 2) (App (Var 2) (Var 0))))) 1 (2+i))
   ) as IH2.
-  { intros op Aop Bop gets. specialize (H3 op Aop Bop gets).
-    specialize (JL _ _ _ H3 A_ins (2+i) wfins) as IH.
+  { intros op Aop Bop gets. specialize (H4 op Aop Bop gets).
+    specialize (JL _ _ _ H4 A_ins (2+i) wfins) as IH.
     clear VL CL HL RL JL WFHL WFFL WFIL.
     simpl in *. auto. }
-  specialize (JL _ _ _ H4 A_ins i) as IH3.
+  specialize (JL _ _ _ H5 A_ins i) as IH3.
   clear VL CL HL RL JL WFHL WFFL WFIL.
   simpl in *. eapply CompInduction; eauto.
+  - apply var_admissible_shift; aomega.
   - rewrite form_shift_subs, <-form_shift_comm, <-hyp_shift_comm in IH1.
     simpl in IH1. all: aomega.
   - intros op Aop Bop gets. specialize (IH2 op Aop Bop gets).
@@ -1179,18 +1180,18 @@ destruct orig. destruct H2.
     simpl. left. auto.
 + eapply CompInduction; eauto.
   - eapply hypotheses_weakening; eauto.
-    apply wf_hyp_shift_typesafe; auto. inv H0. inv H8. inv H7. auto.
+    apply wf_hyp_shift_typesafe; auto. inv H0. inv H9. inv H8. auto.
     apply hyp_subset_shift. auto.
-  - intros op Aop Bop gets. specialize (H3 op Aop Bop gets).
+  - intros op Aop Bop gets. specialize (H4 op Aop Bop gets).
     apply get_op_type_wf in gets. destruct gets.
     eapply hypotheses_weakening; eauto.
     * apply WfHypU. rewrite <-(hyp_shift_shift 1).
       apply wf_hyp_shift_typesafe. apply wf_hyp_shift_typesafe. 
-      3: apply WfTyFun. all: auto. inv H0. inv H10. auto.
-      inv H3. inv H9. auto.
+      3: apply WfTyFun. all: auto. inv H0. inv H11. auto.
+      inv H4. inv H10. auto.
     * apply SubsetHypU. apply hyp_subset_extend. apply hyp_subset_shift. auto.
       simpl. auto.
-    * inv H0. inv H8. inv H7. auto.
+    * inv H0. inv H9. inv H8. auto.
 Qed.
 
 (* ==================== Better Logic Reflexivity. ==================== *)
@@ -1752,7 +1753,7 @@ destruct orig. destruct H2.
   rewrite hyp_shift_sub, form_shift_sub; aomega.
   eapply IH2. eauto. apply v_shift_typesafe; auto.
   inv H2. inv H5. auto.
-+ specialize (JL _ _ _ H2 (S i) (v_shift v_s 1 0) A_s gets) as IH1.
++ specialize (JL _ _ _ H3 (S i) (v_shift v_s 1 0) A_s gets) as IH1.
   assert (
   forall op Aop Bop,
      get_op_type Σ op = Some (Aop, Bop) ->
@@ -1767,28 +1768,29 @@ destruct orig. destruct H2.
              (Fun TyUnit (Op op Aop Bop (Var 2) (App (Var 2) (Var 0)))))
           (2 + i, v_shift v_s 2 0))
   ) as IH2.
-  { intros op Aop Bop gets'. specialize (H3 op Aop Bop gets').
-    specialize (JL _ _ _ H3 (2+i) (v_shift v_s 2 0)) as IH.
+  { intros op Aop Bop gets'. specialize (H4 op Aop Bop gets').
+    specialize (JL _ _ _ H4 (2+i) (v_shift v_s 2 0)) as IH.
     clear VL CL HL RL JL WFHL WFFL WFIL.
     simpl in *. eapply IH; eauto. rewrite <-(v_shift_shift 1).
     apply get_op_type_wf in gets'. destruct gets'.
     apply v_shift_typesafe. apply v_shift_typesafe; auto. 
-    apply WfTyFun; auto. inv H0. inv H10. auto. inv H0. inv H8. inv H7. auto. }
-  specialize (JL _ _ _ H4 i v_s A_s gets) as IH3.
+    apply WfTyFun; auto. inv H0. inv H11. auto. inv H0. inv H9. inv H8. auto. }
+  specialize (JL _ _ _ H5 i v_s A_s gets) as IH3.
   clear VL CL HL RL JL WFHL WFFL WFIL.
-  inv H0. inv H8.
+  inv H0. inv H9.
   simpl in *. eapply CompInduction; eauto.
+  - apply var_admissible_sub; aomega. apply v_shift_makes_no_var.
   - clear IH2. rewrite form_sub_subs in IH1. simpl in IH1.
     rewrite form_shift_sub, v_shift_comm, hyp_shift_sub. 
     simpl in *. all: aomega.
-    apply IH1. apply v_shift_typesafe. auto. inv H7. auto.
+    apply IH1. apply v_shift_typesafe. auto. inv H8. auto.
   - intros op Aop Bop gets'. specialize (IH2 op Aop Bop gets').
     apply get_op_type_wf in gets'. destruct gets'.
     rewrite hyp_shift_sub, form_shift_sub.
     rewrite form_sub_subs, form_sub_subs in IH2.
     simpl in *. rewrite v_shift_shift in IH2. simpl in IH2.
     rewrite form_shift_sub, v_shift_comm, (v_shift_comm 1 0).
-    all: aomega. inv H7. auto.
+    all: aomega. inv H8. auto.
   - rewrite form_sub_subs in IH3. simpl in IH3. auto. omega.
 }{
 intros gets vtys. inv orig.
@@ -2704,7 +2706,7 @@ unfold v_subs. simpl. apply VeqNil; auto.
   rewrite hyp_shift_subs_alt, form_shift_subs_alt; aomega.
   eapply IH2. eauto. apply v_shift_typesafe; eauto.
   inv H2. inv H5. auto. f_equal. auto. omega.
-+ specialize (JL (CtxU Γ A) _ _ _ H2 (S i) ) as IH1.
++ specialize (JL (CtxU Γ A) _ _ _ H3 (S i) ) as IH1.
   assert (
   forall op Aop Bop,
      get_op_type Σ op = Some (Aop, Bop) ->
@@ -2719,25 +2721,26 @@ unfold v_subs. simpl. apply VeqNil; auto.
              (Fun TyUnit
               (Op op Aop Bop (Var 2) (App (Var 2) (Var 0))))) (2 + i) (v_shift v_s 2 0))
   ) as IH2.
-  { intros op Aop Bop gets'. specialize (H3 op Aop Bop gets').
+  { intros op Aop Bop gets'. specialize (H4 op Aop Bop gets').
     specialize 
-      (JL (CtxU (CtxU Γ Aop) (TyFun Bop (CTy A Σ E))) _ _ _ H3 (2+i)) as IH.
+      (JL (CtxU (CtxU Γ Aop) (TyFun Bop (CTy A Σ E))) _ _ _ H4 (2+i)) as IH.
     all: clear VL CL HL RL JL WFHL WFFL WFIL.
     simpl in *. eapply IH; eauto. clear IH1 IH. 
     rewrite <-(v_shift_shift 1).
     apply get_op_type_wf in gets'. destruct gets'.
     apply v_shift_typesafe. apply v_shift_typesafe; eauto. 
-    apply WfTyFun; auto. inv H0. inv H10. auto. inv H0. inv H8. inv H7. auto.
+    apply WfTyFun; auto. inv H0. inv H11. auto. inv H0. inv H9. inv H8. auto.
     do 2 f_equal. auto. omega. }
-  specialize (JL Γ _ _ _ H4 i ) as IH3.
+  specialize (JL Γ _ _ _ H5 i ) as IH3.
   clear VL CL HL RL JL WFHL WFFL WFIL.
-  inv H0. inv H8.
+  inv H0. inv H9.
   simpl in *. eapply CompInduction; eauto.
+  - apply var_admissible_subs; aomega. apply v_shift_makes_no_var.
   - clear IH2. specialize (IH1 (v_shift v_s 1 0) A_s).
     rewrite form_subs_subs in IH1. simpl in IH1. unfold v_subs in IH1.
     rewrite form_shift_subs_alt, v_shift_comm, hyp_shift_subs_alt. 
     simpl in *. all: aomega.
-    apply IH1. apply v_shift_typesafe. auto. inv H7. all: aomega.
+    apply IH1. apply v_shift_typesafe. auto. inv H8. all: aomega.
   - intros op Aop Bop gets'. specialize (IH2 op Aop Bop gets').
     apply get_op_type_wf in gets'. destruct gets'.
     rewrite <-(hyp_shift_shift 1).
@@ -2751,7 +2754,7 @@ unfold v_subs. simpl. apply VeqNil; auto.
     rewrite (form_subs_subs (form_shift φ 2 0)) in IH2.
     rewrite <-(v_shift_comm 1 0 0 3), v_shift_shift in IH2.
     rewrite <-(v_shift_comm 1 0 0 2), v_shift_shift in IH2.
-    unfold v_subs in IH2. simpl in *. all: aomega. inv H7. auto.
+    unfold v_subs in IH2. simpl in *. all: aomega. inv H8. auto.
   - clear IH1 IH2. specialize (IH3 v_s A_s tyvs). 
     rewrite form_subs_subs in IH3. unfold v_subs in IH3. simpl in IH3.
     apply IH3. all: aomega.
